First version of Main all the way to Coarse Asm.

concurrency/common/ClightSemantincsForMachines.v
@@ -1,3 +1,12 @@
+(* Clight SEmantics for Machines*)
+
+(*
+  We define event semantics for 
+  - Clight_new: the core semantics defined by VST
+  - Clightcore: the core semantics derived from 
+    CompCert's Clight
+*)
+
 Require Import compcert.common.Memory.
 
 
@@ -19,6 +28,8 @@ Require Import VST.concurrency.common.permissions.
 (*Semantics*)
 Require Import VST.veric.Clight_new.
 Require Import VST.veric.Clightnew_coop.
+Require Import VST.veric.Clight_core.
+Require Import VST.veric.Clightcore_coop. 
 Require Import VST.sepcomp.event_semantics.
 
 Section ClightSEM.
@@ -30,6 +41,9 @@ Section ClightSEM.
   (* We might want to define this properly or
      factor the machines so we don't need events here. *)
 
+
+
+  (** *Event semantics for Clight_new*)
   (* This should be a version of CLN_memsem annotated with memory events. *)
   Program Definition CLN_evsem ge : @EvSem C := {| msem := CLN_memsem ge |}.
   Next Obligation.
@@ -46,24 +60,48 @@ Section ClightSEM.
   Lemma CLN_msem : forall ge, msem (CLN_evsem ge) = CLN_memsem ge.
   Proof. auto. Qed.
 
-  Notation Sem := CLN_evsem.
-  Lemma step_decay: forall g c m tr c' m',
-      event_semantics.ev_step (Sem g) c m tr c' m' ->
+  Lemma CLN_step_decay: forall g c m tr c' m',
+      event_semantics.ev_step (CLN_evsem g) c m tr c' m' ->
       decay m m'.
   Admitted.
 
   Lemma initial_core_mem_congr: forall n ge m m' q v vl,
-    initial_core (Sem ge) n m q v vl <-> initial_core (Sem ge) n m' q v vl.
+    initial_core (CLN_evsem ge) n m q v vl <-> initial_core (CLN_evsem ge) n m' q v vl.
   Proof. reflexivity. Qed.
 
   Lemma at_external_SEM_eq:
-     forall ge c m, at_external (Sem ge) c m =
+     forall ge c m, at_external (CLN_evsem ge) c m =
       match c with
       | State _ _ _ => None
       | ExtCall ef args _ _ _ _ => Some (ef, args)
       end.
   Proof. auto. Qed.
 
-  Instance ClightSem ge : Semantics := { semG := G; semC := C; semSem := CLN_evsem ge; the_ge := ge }.
+  Instance Clight_newSem ge : Semantics :=
+    { semG := G; semC := C; semSem := CLN_evsem ge; the_ge := ge }.
 
+  
+
+
+  (** *Event semantics for Clight_new*)
+  (* This should be a version of CLN_memsem annotated with memory events. *)
+  Program Definition CLC_evsem ge : @EvSem state := {| msem := CLC_memsem ge |}.
+  Next Obligation.
+  Admitted.
+  Next Obligation.
+  Admitted.
+  Next Obligation.
+  Admitted.
+  Next Obligation.
+  Admitted.
+  Next Obligation.
+  Admitted.
+
+  Lemma CLC_msem : forall ge, msem (CLC_evsem ge) = CLC_memsem ge.
+  Proof. auto. Qed.
+
+
+  Instance ClightSem ge : Semantics :=
+    { semG := G; semC := state; semSem := CLC_evsem ge; the_ge := ge }.
+  
 End ClightSEM.
