concurrency/common/HybridMachine.v
@@ -714,4 +714,5 @@ Module DryHybridMachine.
     
   End DryHybridMachine.
 End DryHybridMachine.
+Set Printing All.
 Export DryHybridMachine.
